rename ASubstitution.comp into sub_comp, fill_comp into fill_fill, sub_comp_single into sub_comp_single_extend, and app_comp_single into sub_comp_single moved from AUnif to ASubstitution

trunk/color/Term/WithArity/AContext.v
@@ -14,6 +14,10 @@ Require Import LogicUtil.
 Require Export ATerm.
 Require Import VecUtil.
 Require Import ListUtil.
+Require Import LogicUtil.
+Require Import EqUtil.
+Require Import BoolUtil.
+Require Import VecUtil.
 
 Section S.
 
@@ -38,12 +42,27 @@ Fixpoint fill (c : context) (t : term) {struct c} : term :=
   end.
 
 (***********************************************************************)
+(** context composition *)
+
+Fixpoint comp (C : context) : context -> context :=
+  match C with
+    | Hole => fun E => E
+    | Cont _ _ _ H ts1 D ts2 => fun E => Cont H ts1 (comp D E) ts2
+  end.
+
+Lemma fill_fill : forall C D u, fill C (fill D u) = fill (comp C D) u.
+
+Proof.
+induction C; simpl; intros. refl. rewrite (IHC D u). refl.
+Qed.
+
+(***********************************************************************)
 (** properties of fill *)
 
 Lemma var_eq_fill : forall x c t, Var x = fill c t -> c = Hole /\ t = Var x.
 
 Proof.
-intros. destruct c; simpl in H. auto. discriminate.
+intros. destruct c; simpl in H. auto. discr.
 Qed.
 
 Lemma fun_eq_fill : forall f ts c u, Fun f ts = fill c u ->
@@ -94,17 +113,17 @@ Proof.
 intros. unfold subterm.
 assert (exists n1, exists v1 : terms n1, exists n2, exists v2 : terms n2,
   exists H : n1 + S n2 = arity f, ts = Vcast (Vapp v1 (Vcons u v2)) H).
-apply Vin_elim. assumption.
+apply Vin_elim. hyp.
 destruct H0 as [n1]. destruct H0 as [ts1].
 destruct H0 as [n2]. destruct H0 as [ts2]. destruct H0 as [H1].
-exists (Cont H1 ts1 Hole ts2). split. discriminate.
+exists (Cont H1 ts1 Hole ts2). split. discr.
 rewrite H0. refl.
 Qed.
 
 Lemma subterm_strict : forall u t, subterm u t -> subterm_eq u t.
 
 Proof.
-unfold subterm_eq, subterm. intros. destruct H. destruct H. exists x. assumption.
+unfold subterm_eq, subterm. intros. destruct H. destruct H. exists x. hyp.
 Qed.
 
 Lemma subterm_noteq : forall u t, subterm_eq u t -> u <> t -> subterm u t.
@@ -112,23 +131,7 @@ Lemma subterm_noteq : forall u t, subterm_eq u t -> u <> t -> subterm u t.
 Proof.
 unfold subterm_eq, subterm. intros. destruct H as [C]. destruct C.
 subst t. simpl in H0. absurd (u<>u); auto.
-exists (Cont e v C v0). split. discriminate. subst t. refl.
-Qed.
-
-(***********************************************************************)
-(** context composition *)
-
-Fixpoint comp (C : context) : context -> context :=
-  match C with
-    | Hole => fun E => E
-    | Cont _ _ _ H ts1 D ts2 => fun E => Cont H ts1 (comp D E) ts2
-  end.
-
-Lemma fill_comp : forall C D u, fill C (fill D u) = fill (comp C D) u.
-
-Proof.
-induction C; simpl; intros. refl.
-rewrite (IHC D u). refl.
+exists (Cont e v C v0). split. discr. subst t. refl.
 Qed.
 
 (***********************************************************************)
@@ -139,8 +142,8 @@ Lemma subterm_trans_eq1 : forall t u v,
 
 Proof.
 unfold subterm, subterm_eq. intros. destruct H. destruct H0. destruct H0.
-subst u. subst v. rewrite (fill_comp x0 x t). exists (comp x0 x).
-split. destruct x0. absurd (Hole = Hole); auto. simpl. discriminate. refl.
+subst u. subst v. rewrite (fill_fill x0 x t). exists (comp x0 x).
+split. destruct x0. absurd (Hole = Hole); auto. simpl. discr. refl.
 Qed.
 
 Lemma subterm_trans_eq2 : forall t u v,
@@ -148,9 +151,9 @@ Lemma subterm_trans_eq2 : forall t u v,
 
 Proof.
 unfold subterm, subterm_eq. intros. destruct H. destruct H. destruct H0.
-subst u. subst v. rewrite (fill_comp x0 x t). exists (comp x0 x).
+subst u. subst v. rewrite (fill_fill x0 x t). exists (comp x0 x).
 split. destruct x. absurd (Hole = Hole); auto.
-destruct x0; simpl; discriminate. refl.
+destruct x0; simpl; discr. refl.
 Qed.
 
 Lemma subterm_trans : forall t u v,
@@ -158,9 +161,17 @@ Lemma subterm_trans : forall t u v,
 
 Proof.
 unfold subterm. intros. do 2 destruct H. do 2 destruct H0.
-subst u. subst v. rewrite (fill_comp x0 x t). exists (comp x0 x).
+subst u. subst v. rewrite (fill_fill x0 x t). exists (comp x0 x).
 split. destruct x. absurd (Hole = Hole); auto.
-destruct x0; simpl; discriminate. refl.
+destruct x0; simpl; discr. refl.
+Qed.
+
+Lemma subterm_eq_trans : forall t u v,
+  subterm_eq t u -> subterm_eq u v -> subterm_eq t v.
+
+Proof.
+intros. destruct H. destruct H0. subst. rewrite fill_fill.
+exists (comp x0 x). refl.
 Qed.
 
 (***********************************************************************)
@@ -171,9 +182,9 @@ Lemma subterm_eq_vars : forall u t x,
 
 Proof.
 unfold subterm_eq. intros. destruct H as [C]. subst t. elim C; clear C.
-simpl. assumption. intros. simpl fill. rewrite vars_fun.
+simpl. hyp. intros. simpl fill. rewrite vars_fun.
 rewrite vars_vec_cast. rewrite vars_vec_app. rewrite vars_vec_cons.
-apply in_appr. apply in_appl. assumption.
+apply in_appr. apply in_appl. hyp.
 Qed.
 
 Lemma in_vars_subterm_eq : forall x t, In x (vars t) -> subterm_eq (Var x) t.
@@ -185,7 +196,7 @@ generalize (in_vars_vec_elim H0). intro.
 destruct H1 as [t]. destruct H1. generalize (Vforall_in H H1). intro.
 generalize (H3 H2). intro. apply subterm_strict. eapply subterm_trans_eq1.
 apply H4.
-apply subterm_fun. assumption.
+apply subterm_fun. hyp.
 Qed.
 
 Lemma in_vars_fun : forall x f ts,
@@ -193,7 +204,7 @@ Lemma in_vars_fun : forall x f ts,
 
 Proof.
 intros. apply subterm_fun_elim. ded (in_vars_subterm_eq _ _ H).
-apply subterm_noteq. assumption. discriminate.
+apply subterm_noteq. hyp. discr.
 Qed.
 
 (***********************************************************************)
@@ -214,17 +225,17 @@ Proof.
 intros P IH. set (P' := fun t => forall u, subterm_eq u t -> P u).
 change (forall t, P' t). apply term_ind_forall.
 (* var *)
-unfold P'. intros. assert (u = Var v). apply subterm_eq_var. assumption.
+unfold P'. intros. assert (u = Var v). apply subterm_eq_var. hyp.
 subst u. apply IH. unfold subterm. intros. destruct H0. destruct H0.
-destruct x. absurd (Hole = Hole); auto. discriminate.
+destruct x. absurd (Hole = Hole); auto. discr.
 (* fun *)
 intros. unfold P'. intros. apply IH. intros.
-assert (subterm u0 (Fun f v)). eapply subterm_trans_eq2. apply H1. assumption.
+assert (subterm u0 (Fun f v)). eapply subterm_trans_eq2. apply H1. hyp.
 assert (exists t, Vin t v /\ subterm_eq u0 t). apply subterm_fun_elim.
-assumption.
+hyp.
 destruct H3. destruct H3.
-assert (P' x). eapply Vforall_in with (n := arity f). apply H. assumption.
-apply H5. assumption.
+assert (P' x). eapply Vforall_in with (n := arity f). apply H. hyp.
+apply H5. hyp.
 Qed.
 
 Lemma subterm_ind : forall (P : term -> Prop)
@@ -232,8 +243,39 @@ Lemma subterm_ind : forall (P : term -> Prop)
   forall t, P t.
 
 Proof.
-intros. apply forall_subterm_eq. apply subterm_ind_sub. assumption.
+intros. apply forall_subterm_eq. apply subterm_ind_sub. hyp.
 Qed.
+
+(***********************************************************************)
+(** boolean function for testing subterm *)
+
+Fixpoint bsubterm_eq (t u : term) {struct u} : bool :=
+  match u with
+    | Var _ => beq_term t u
+    | Fun _ us => beq_term t u || bVexists (bsubterm_eq t) us
+  end.
+
+Lemma bsubterm_eq_ok : forall t u, bsubterm_eq t u = true <-> subterm_eq t u.
+
+Proof.
+intros t u. pattern u; apply term_ind_forall; clear u; simpl.
+(* Var *)
+intro. rewrite beq_term_ok. split; intro. subst. apply subterm_eq_refl.
+apply subterm_eq_var in H. hyp.
+(* Fun *)
+split; rewrite orb_eq; rewrite beq_term_ok; intros. destruct H0.
+subst. apply subterm_eq_refl. rewrite bVexists_ok_Vin in H0.
+Focus 2. intros. pattern x. apply Vforall_in with (v:=v). apply H. hyp.
+rewrite Vexists_eq in H0. decomp H0. apply subterm_eq_trans with x.
+hyp. apply subterm_strict. apply subterm_fun. hyp.
+
+Abort.
+
+Definition bsubterm (t u : term) : bool :=
+  match u with
+    | Var x => false
+    | Fun _ us => bVexists (bsubterm_eq t) us
+  end.
 
 (***********************************************************************)
 (** variables of a context *)
@@ -261,7 +303,8 @@ Lemma vars_fill_intro : forall t c, incl (cvars c ++ vars t) (vars (fill c t)).
 Proof.
 induction c. simpl. apply incl_refl. simpl cvars. simpl fill. rewrite vars_fun.
 rewrite vars_vec_cast. rewrite vars_vec_app. rewrite vars_vec_cons.
-rewrite app_ass. apply appl_incl. apply app_com_incl. apply appr_incl. exact IHc.
+rewrite app_ass. apply appl_incl. apply app_com_incl. apply appr_incl.
+exact IHc.
 Qed.
 
 End S.
